
>Let $\mathcal{P}$ and $\mathcal{Q}$ be the physical and risk neutral measures on $(\omega,\mathcal{F})$ respectively. Let $\{W_t^\mathcal{P}\}_{t \geq 0}$ be the standard Brownian motion on $\mathcal{P}$. For $\{S_t\}_{t \geq 0}$ be the process of asset price, we have:
$$dSt = 0.15St \,dt + 0.4 S_t \,dW_t^\mathcal{P}$$

>With $f(t,x)=e^{-0.06t}x$ then we can calculate:
$$\begin{align*} 
f_t&=-0.06e^{-0.06t}x \\
f_x&=e^{-0.06t} \\
f_{tt}&=0.06^2e^{-0.06t}x \\
f_{xx}&=0 \\
f_{tx}&=0
\end{align*}$$

>Aply Ito-Doeblin formula, we have:
$$\begin{align*}
d(e^{-0.06t}S_t) &= -0.06e^{-0.06t}S_t\,dt+e^{-0.06t}\,dS_t \\
&= -0.06e^{-0.06t}S_t\,dt+e^{-0.06t}(0.15St \,dt + 0.4 S_t \,dW_t^\mathcal{P}) \\
&= e^{-0.06t}S_t[(-0.06+0.15) \,dt+0.4 \,d W_t^{\mathcal{P}}] \\
&= e^{-0.06t}S_t[-0.06+0.15 \,dt+0.4 (\,d W_t^{\mathcal{Q}}-\theta_t) \,dt] \\
&= e^{-0.06t}S_t[(-0.06+0.15-0.4 \theta_t) \,dt+0.4 \,d W_t^{\mathcal{Q}} \,dt]
\end{align*}$$

>In order to have the process $\{e^{−0.06t}S_t\}_{t \geq 0}$ be the martigale process, we choose $\theta_t$ such that:
$$-0.06+0.15-0.4 \theta_t=0 \rightarrow \theta_t=\frac{-0.06+0.15}{0.4} $$
then $$E^\mathcal{P}[e^{\frac{1}{2} \int_0^T \theta_t^2\,dt}]<\infty$$

>By the Girsanov’s theorem, there is a risk neutral measure $\mathcal{Q}$ defined by the Radon-Nykodym $$E \left[\frac{\,d \mathcal{Q}}{\,d \mathcal{P}} |\mathcal{F}_t\right]=Z_t=e^{-\int_0^t \theta_s \,d W_s^\mathcal{P}-\frac{1}{2} \theta_s^2 \,ds}$$ such that $W_t^\mathcal{Q}=W_t^\mathcal{P}+\int_0^t\theta_s \,ds$  
is the standard Brownian motion under $\mathcal{Q}$.
$$W_t^\mathcal{Q}=W_t^\mathcal{P}+\int_0^t\theta_s \,ds \\
\rightarrow \,dW_t^\mathcal{Q}=\,dW_t^\mathcal{P}+\theta_t\,dt$$

>Since $e^{-rt}S_t$ is a martingale under $\mathcal{Q}$ and $\mathcal{Q}$ is an equivalent martingale measure to $\mathcal{P}$, we can write:
$$\begin{align*}
\,dSt &= 0.15St \,dt + 0.4 S_t \,dW_t^\mathcal{P} \\
&=0.15St \,dt + 0.4 S_t (\,dW_t^\mathcal{Q}-\theta_t \,dt) \\
&=0.15St \,dt + 0.4 S_t (\,dW_t^\mathcal{Q}-\frac{-0.06+0.15}{0.4} \,dt) \\
&=\left(0.15-0.4\times\frac{-0.06+0.15}{0.4} \right)St \,dt + 0.4 S_t \,dW_t^\mathcal{Q} \\
&=-0.06St \,dt + 0.4 S_t \,dW_t^\mathcal{Q} \\
\end{align*}$$

>Let $Y_t=\ln S_t$ and $f(t,x)=\ln x$, we have:
$$\begin{align*}
f_t&=0 \\
f_x&=\frac{1}{x} \\
f_{tt}&=0 \\
f_{xx}&=-\frac{1}{x^2} \\
f_{tx}&=0 \\
\end{align*}$$

>Applying Ito Doeblin formula, we have:
$$\begin{align*}
\,d(Y_t)&=\frac{1}{S_t} \,dS_t-\frac{1}{2}\frac{1}{S_t^2}\,dS_t^2 \\
&=\frac{1}{S_t} (0.06St \,dt + 0.4 S_t \,dW_t^\mathcal{Q})-\frac{1}{2}\frac{1}{S_t^2}(0.06St \,dt + 0.4 S_t \,dW_t^\mathcal{Q})^2 \\
&=(0.06-\frac{1}{2} \times 0.4^2)\,dt + 0.4 \,dW_t^\mathcal{Q} \\
\,d(\ln S_t)&=(0.06-\frac{1}{2} \times 0.4^2)\,dt + 0.4 \,dW_t^\mathcal{Q} \\
 \int_t^T \,d(\ln S_s)&=\int_t^T(0.06-\frac{1}{2} \times 0.4^2)\,ds + \int_t^T0.4 \,dW_s^\mathcal{Q} \\
 ln \left( \frac{S_T}{S_t} \right)&=(0.06-\frac{1}{2} \times 0.4^2)(T-t)+0.4(W_T^\mathcal{Q}-W_t^\mathcal{Q}) \\
 S_T&=e^{\ln S_t +(0.06-\frac{1}{2} \times 0.4^2)(T-t)+0.4(W_T^{\mathcal{Q}}-W_t^{\mathcal{Q}})}
\end{align*}$$

2. Compute the fair price when $t = 0.5,T = 1, S_t = 10$.

>We have
$$\begin{align*}
\ln S_t +(0.06-\frac{1}{2} \times 0.4^2)(T-t)+0.4(W_T^{\mathcal{Q}}-W_t^{\mathcal{Q}}) &\sim \mathcal{N}(\ln S_t +(0.06-\frac{1}{2} \times 0.4^2)(T-t),0.4^2(T-t)) \\
e^{\ln S_t +(0.06-\frac{1}{2} \times 0.4^2)(T-t)+0.4(W_T^{\mathcal{Q}}-W_t^{\mathcal{Q}})} &\sim \log \mathcal{N}(\ln S_t +(0.06-\frac{1}{2} \times 0.4^2)(T-t),0.4^2(T-t)) \\
 (S_T|S_t) &\sim \log \mathcal{N}(\ln S_t +(0.06-\frac{1}{2} \times 0.4^2)(T-t),0.4^2(T-t)) \\
\end{align*}$$

>The probability density function of $(S_T|S_t)$ is
$$f_{S_T|S_t}(x)=\frac{1}{0.4x\sqrt{2\pi(T-t)}}e^{-\frac{1}{2} \frac{(\ln x-(\ln S_t +(0.06-\frac{1}{2} \times 0.4^2)(T-t)))^2}{0.4^2(T-t)}} $$

>From Feyman-Kac formula we have:
$$ C(S_t,t)=e^{-0.06(T-t)} \mathbb{E}^\mathcal{Q}[max(S_T-K,0)|\mathcal{F}_t] $$

>Applying the moment generating function, we have:
$$\begin{align*} 
C(S_t,t)&=e^{-0.06(T-t)}\int_{-\infty}^\infty \max(x-8,0) f_{S_T|S_t}(x) \,dx \\
C(S_t,t)&=e^{-0.06(T-t)}\int_8^\infty (x-8) \frac{1}{0.4x\sqrt{2\pi}\sqrt{(T-t)}}e^{-\frac{1}{2} \frac{(\ln x-(\ln S_t +(0.06-\frac{1}{2} \times 0.4^2)(T-t)))^2}{0.4^2(T-t)}} \,dx
\end{align*}$$

>With the maturity time $T=1$, substitute $S_t=10$ and $t=0.5$, we have
$$\begin{align*}
C(10,0.5)&=e^{-0.06(1-0.5)}\int_8^\infty (x-8) \frac{1}{0.4x\sqrt{2\pi}\sqrt{(1-0.5)}}e^{-\frac{1}{2} \frac{(\ln x-(\ln 10 +(0.06-\frac{1}{2} \times 0.4^2)(1-0.5)))^2}{0.4^2(1-0.5)}} \,dx \\
&=\frac{e^{-0.06(1-0.5)}}{0.4 \sqrt{2\pi}\sqrt{(1-0.5)}} \int_8^\infty (x-8)e^{-\frac{1}{2} \frac{(\ln x-\ln 10 -(0.06-\frac{1}{2} \times 0.4^2)(1-0.5)))^2}{0.4^2(1-0.5)}} \frac{1}{x}\,dx
\end{align*}$$

>Let $u_x=\frac{\ln x-\ln 10 -(0.06-\frac{1}{2} \times 0.4^2)(1-0.5)}{0.4\sqrt{1-0.5}}$, we have
$$\begin{align*}
\ln \left( \frac{x}{10} \right)&=0.4u\sqrt{1-0.5}+(0.06-\frac{1}{2} \times 0.4^2)(1-0.5) \\
x&=10e^{0.4u\sqrt{1-0.5}+(0.06-\frac{1}{2} \times 0.4^2)(1-0.5)}
\end{align*}$$ 

>$$\begin{align*}
\,du&=\frac{1}{0.4x\sqrt{1-0.5}}\,dx \\
0.4\sqrt{1-0.5}\,du&=\frac{1}{x}\,dx
\end{align*}$$

>$$\begin{align*}
u_8&=\frac{\ln 8-\ln 10 +(0.06-\frac{1}{2} \times 0.4^2)(1-0.5)}{0.4\sqrt{1-0.5}} \\
&=\frac{\ln \left( \frac{8}{10} \right)+(0.06-\frac{1}{2} \times 0.4^2)(1-0.5)}{0.4\sqrt{1-0.5}}
\end{align*}$$

>The value of the call option becomes:
$$\begin{align*}
    C(10,0.5)&=\frac{e^{-0.06(1-0.5)}}{0.4 \sqrt{2\pi} \sqrt{T-t}} \int_8^\infty (x-8)e^{-\frac{1}{2} \frac{(\ln x-\ln 10 -(0.06-\frac{1}{2} \times 0.4^2)(1-0.5)))^2}{0.4^2(1-0.5)}} \frac{1}{x}\,dx \\
    &=\frac{e^{-0.06(1-0.5)}}{0.4 \sqrt{2\pi}\sqrt{T-t}} \int_{u_8}^\infty (10e^{0.4u\sqrt{1-0.5}+(0.06-\frac{1}{2} \times 0.4^2)(1-0.5)}-8)e^{-\frac{1}{2} u^2} 0.4\sqrt{1-0.5}\,du \\
    &=\frac{e^{-0.06(1-0.5)}\sqrt{1-0.5}}{\sqrt{2\pi}\sqrt{T-t}} \int_{u_8}^\infty (10e^{0.4u\sqrt{1-0.5}+(0.06-\frac{1}{2} \times 0.4^2)(1-0.5)}e^{-\frac{1}{2} u^2}-8e^{-\frac{1}{2} u^2}) \,du \\
    &=\frac{e^{-0.06(1-0.5)}}{\sqrt{2\pi}} \int_{u_8}^\infty (10e^{0.4u\sqrt{1-0.5}+(0.06-\frac{1}{2} \times 0.4^2)(1-0.5)-\frac{1}{2} u^2}-8e^{-\frac{1}{2} u^2}) \,du \\
    &=\frac{e^{-0.06(1-0.5)}}{\sqrt{2\pi}} \int_{u_8}^\infty 10e^{0.4u\sqrt{1-0.5}+(0.06-\frac{1}{2} \times 0.4^2)(1-0.5)-\frac{1}{2} u^2}\,du-\frac{e^{-0.06(1-0.5)}}{\sqrt{2\pi}} \int_{u_8}^\infty 8e^{-\frac{1}{2} u^2} \,du \\
    &=\frac{10}{\sqrt{2\pi}} \int_{u_8}^\infty e^{-\frac{1}{2} u^2+0.4u\sqrt{1-0.5}-0.06(1-0.5)+(0.06-\frac{1}{2} \times 0.4^2)(1-0.5)}\,du-\frac{8e^{-0.06(1-0.5)}}{\sqrt{2\pi}} \int_{u_8}^\infty e^{-\frac{1}{2} u^2} \,du \\
    &=\frac{10}{\sqrt{2\pi}} \int_{u_8}^\infty e^{-\frac{1}{2} (u-0.4\sqrt{1-0.5})^2}\,du-\frac{8e^{-0.06(1-0.5)}}{\sqrt{2\pi}} \int_{u_8}^\infty e^{-\frac{1}{2} u^2} \,du \\
    &=\frac{10}{\sqrt{2\pi}} \int_{u_8}^\infty e^{-\frac{1}{2} (u-0.4\sqrt{1-0.5})^2}\,d(u-0.4\sqrt{1-0.5})-\frac{8e^{-0.06(1-0.5)}}{\sqrt{2\pi}} \int_{u_8}^\infty e^{-\frac{1}{2} u^2} \,du \\
    &=\frac{10}{\sqrt{2\pi}} \int_{u_8-0.4\sqrt{1-0.5}}^\infty e^{-\frac{1}{2} u^2}\,du-\frac{8e^{-0.06(1-0.5)}}{\sqrt{2\pi}} \int_{u_8}^\infty e^{-\frac{1}{2} u^2} \,du \\
    &= \frac{10}{\sqrt{2\pi}} \int_{-\infty}^{0.4\sqrt{1-0.5}-u_8} e^{-\frac{1}{2} u^2}\,du-\frac{8e^{-0.06(1-0.5)}}{\sqrt{2\pi}} \int_{-\infty}^{-u_8} e^{-\frac{1}{2} u^2} \,du \\
    &=10\times \frac{1}{\sqrt{2\pi}} \int_{-\infty}^{0.4\sqrt{1-0.5}-\frac{\ln \left( \frac{8}{10} \right)-(0.06-\frac{1}{2} \times 0.4^2)(1-0.5)}{0.4\sqrt{1-0.5}}} e^{-\frac{1}{2} u^2}\,du-8e^{-0.06(1-0.5)} \times \frac{1}{\sqrt{2\pi}} \int_{-\infty}^{-\frac{\ln \left( \frac{8}{10} \right)-(0.06-\frac{1}{2} \times 0.4^2)(1-0.5)}{0.4\sqrt{1-0.5}}} e^{-\frac{1}{2} u^2} \,du \\
    &=10\times \frac{1}{\sqrt{2\pi}} \int_{-\infty}^{\frac{\ln \left( \frac{10}{8} \right)+(0.06+\frac{1}{2} \times 0.4^2)(1-0.5)}{0.4\sqrt{1-0.5}}} e^{-\frac{1}{2} u^2}\,du-8e^{-0.06(1-0.5)} \times \frac{1}{\sqrt{2\pi}} \int_{-\infty}^{\frac{\ln \left( \frac{10}{8} \right)+(0.06-\frac{1}{2} \times 0.4^2)(1-0.5)}{0.4\sqrt{1-0.5}}} e^{-\frac{1}{2} u^2} \,du \\
    &=10 \times N \left({\frac{\ln \left( \frac{10}{8} \right)+(0.06+\frac{1}{2} \times 0.4^2)(1-0.5)}{0.4\sqrt{1-0.5}}}\right) -8e^{-0.06(1-0.5)} \times N \left({\frac{\ln \left( \frac{10}{8} \right)+(0.06-\frac{1}{2} \times 0.4^2)(1-0.5)}{0.4\sqrt{1-0.5}}}\right)
    \end{align*}$$